post-rebase fixes

Kraken/Semantics.lean
@@ -428,8 +428,8 @@ def Operation.interp [Labels] [address_size : AddressSize]
   | .pop dst =>
     let rsp := s.regs.get64 .rsp
     s.simple_load rsp w (fun val =>
-    s.set dst val p (fun s =>
-    next { s with regs := s.regs.set64 .rsp (rsp + w.bytesv) }))
+    let s := { s with regs := s.regs.set64 .rsp (rsp + w.bytesv) }
+    s.set dst val p next)
   | .setcc cc dst =>
     s.set dst (cc.interp s.status) p next
   | .cmovcc cc dst src =>
@@ -551,7 +551,7 @@ def Operation.interp [Labels] [address_size : AddressSize]
       let low := result.take w.bits
       let high := (result.drop w.bits).setWidth _
       (s.setReg (.low .rax w) low).setReg (.low .rdx w) high
-    undefined (λ sf => undefined (λ zf => undefined (λ af => undefined (λ pf =>
+    pick Bool (λ sf => pick Bool (λ zf => pick Bool (λ af => pick Bool (λ pf =>
     let low := BitVec.ofInt w.bits v
     let cf := v != low.toInt
     next { s with status := { cf := cf, pf, af, zf, sf, of := cf }})))))
