Kraken/Examples/Examples.lean
@@ -220,15 +220,21 @@ example [layout : Layout] s : step1 (layout p4) (s, layout.start) (fun s => s.1.
   dsimp only [step1,Executable.straightline]
   rw [Executable.directivesFromStart]
   simp [List.mapIdx,List.mapIdx.go]
-  dsimp (zeta:=false) only [Directives.interp,Directive.interp,Instr.interp,Operation.interp,Operand.interp,ConstExpr.interp,RegOrMem.interp,Reg.interp,Reg64s.get,Reg.base,Reg.offset,MachineData.set,MachineData.setReg,Reg64s.set,Width.type,Width.bits]
+  dsimp (zeta:=false)(iota:=true) only [Directives.interp,Directive.interp,Instr.interp,Operation.interp,Operand.full_interp,ConstExpr.interp,RegOrMem.interp,Reg.interp,Reg64s.get,Reg.base,Reg.offset,MachineData.set,MachineData.setReg,Reg64s.set,Width.type,Width.bits,Effects.all]
+  simp only [reduceIte]
+  dsimp (zeta:=false)(iota:=true) only [Directives.interp,Directive.interp,Instr.interp,Operation.interp,Operand.full_interp,ConstExpr.interp,RegOrMem.interp,Reg.interp,Reg64s.get,Reg.base,Reg.offset,MachineData.set,MachineData.setReg,Reg64s.set,Width.type,Width.bits,Effects.all]
+  simp only [reduceIte]
+  dsimp (zeta:=false)(iota:=true) only [Directives.interp,Directive.interp,Instr.interp,Operation.interp,Operand.full_interp,ConstExpr.interp,RegOrMem.interp,Reg.interp,Reg64s.get,Reg.base,Reg.offset,MachineData.set,MachineData.setReg,Reg64s.set,Width.type,Width.bits,Effects.all]
   dsimp (zeta:=false)(beta:=true)(eta:=false)(iota:=true)(proj:=true) only [Reg64s.get64,Reg64s.set64,BitVec.drop,BitVec.take,ss] -- reduces UInt64.toBitVec but leaves let binders behind and gets stuck confused on it
+  lift_lets
+  dsimp (zeta:=false)(beta:=true)(eta:=false)(iota:=true)(proj:=true) only [Reg64s.get64,Reg64s.set64,BitVec.drop,BitVec.take,ss] -- reduces UInt64.toBitVec but leaves let binders behind and gets stuck confused on it
+  intros t
   intros rax1
-  lift_lets; intros t -- unfortunately a separte tactic rather than a simp flag
+  -- lift_lets; intros t -- unfortunately a separte tactic rather than a simp flag
   -- simp [MachineData.regs,Reg64s.set64,Reg64s.get64,ss] at t -- made no progress for some reason
-  dsimp (zeta:=false)(beta:=false)(eta:=false)(iota:=false)(proj:=true) only [Reg64s.set64,Reg64s.get64,ss,t]
+  -- dsimp (zeta:=false)(beta:=false)(eta:=false)(iota:=false)(proj:=true) only [Reg64s.set64,Reg64s.get64,ss,t]
   -- now just bashing because rax1 in context is already bad
-  simp [rax1]
+  simp [rax1,t]
   simp (ground:=true)
   simp
   simp (decide:=true)
-  
